ModalLogic/complete/Syntax.v
@@ -1,6 +1,5 @@
 Require Import Logic.GeneralLogic.Base.
 Require Import Logic.MinimunLogic.Syntax.
-Require Import Logic.PropositionalLogic.Syntax.
 
 Class ModalLanguage (L: Language): Type := {
   boxp : expr -> expr;
@@ -9,11 +8,24 @@ Class ModalLanguage (L: Language): Type := {
 Definition negp {L: Language} {MinL: MinimunLanguage L}{mL: ModalLanguage L} (x: expr): expr := impp x falsep.
 Definition diamondp {L: Language} {minL: MinimunLanguage L} {mL: ModalLanguage L}: expr -> expr :=
   fun x => negp (boxp (negp x)).
+Definition orp {L: Language} {MinL: MinimunLanguage L}{mL: ModalLanguage L} (l1 l2 : expr): expr :=
+  impp (negp l1) l2.
+Definition andp {L: Language} {MinL: MinimunLanguage L}{mL: ModalLanguage L}(l1 l2 : expr): expr :=
+  negp (orp (negp l1) (negp l2)).
+Definition iffp {L: Language} {MinL: MinimunLanguage L}{mL: ModalLanguage L}(l1 l2 : expr): expr :=
+  andp (impp l1 l2)(impp l2 l1).
+Definition truep {L: Language} {MinL: MinimunLanguage L}{mL: ModalLanguage L}: expr := negp falsep.
 
 Module ModalLanguageNotation.
 
 Notation "□ x" := (boxp x) (at level 35) : syntax. (* Unicode 25a1 *)
 Notation "◇ x" := (diamondp x) (at level 35) : syntax. (* Unicode 25c7 *)
 Notation "~~ x" := (negp x) (at level 35) : syntax.
+Notation "x && y" := (andp x y)(at level 40, left associativity).
+Notation "x <--> y" := (iffp x y) (at level 60, no associativity).
+Reserved Notation "|-- P " (at level 71, no associativity).
+Notation "x --> y" := (impp x y)(at level 55, right associativity).
+Notation "x || y" := (orp x y)(at level 50, left associativity).
+
 End ModalLanguageNotation.
 
